Add show instances for system F types and terms.

coq/SystemFTest.v
@@ -1,1 +1,90 @@
 From QuickChick Require Import QuickChick.
+Import QcDefaultNotation. Open Scope qc_scope.
+Import GenLow GenHigh.
+Set Warnings "-extraction-opaque-accessed,-extraction".
+
+From Coq Require Import
+     ZArith
+     String
+     List.
+
+Require Import SystemF.
+Import ListNotations.
+
+Variant Precedence :=
+| PrecOuter
+| PrecMult
+| PrecAdd
+| PrecSub
+| PrecApp
+| PrecInner
+.
+
+Definition prec_value (p : Precedence) : N :=
+  match p with
+  | PrecOuter => 0
+  | PrecAdd => 1
+  | PrecSub => 1
+  | PrecMult => 2
+  | PrecApp => 3
+  | PrecInner => 4
+  end.
+
+Definition parens (outer inner : Precedence) (s : string) :=
+  if N.leb (prec_value outer) (prec_value inner)
+  then s
+  else "(" ++ s ++ ")".
+
+Definition intersperse (sep : string) (l : list string) : string
+  := fold_left (fun acc s => if eqb "" acc then s else s ++ sep ++ acc) l "".
+
+Fixpoint showFType_helper {I} `{FInt I} `{Show I} (prec : Precedence) (t : FType) :=
+  match t with
+  | Arrow a b => parens prec PrecApp (showFType_helper PrecInner a ++ "->" ++ showFType_helper PrecApp b)
+  | Prod ts => "<" ++ intersperse ", " (map (showFType_helper PrecOuter) ts) ++ ">"
+  | TForall t => parens prec PrecOuter ("forall " ++ showFType_helper PrecOuter t)
+  | TVar x => show x
+  | IntType => "Int"
+  end.
+
+Instance showFType {I} `{FInt I} `{Show I} : Show FType := 
+  {| show := showFType_helper PrecOuter
+  |}.
+
+Instance showPrimOp : Show PrimOp :=
+  {| show :=
+       fun (op : PrimOp) =>
+         match op with
+         | Mul => "*"
+         | Add => "+"
+         | Sub => "-"
+         end
+  |}.
+
+Definition op_prec (op : PrimOp) : Precedence
+  := match op with
+     | Mul => PrecMult
+     | Add => PrecAdd
+     | Sub => PrecSub
+     end.           
+
+Fixpoint showTerm_helper {I} `{FInt I} `{Show I} (prec : Precedence) (e : Term) :=
+  match e with
+  | Var x => show x
+  | Ann e t => parens prec PrecOuter (showTerm_helper PrecOuter e ++ " : " ++ show t)
+  | Fix t body => parens prec PrecOuter ("λ " ++ show t ++ ". " ++ showTerm_helper PrecOuter body)
+  | TAbs e => parens prec PrecOuter ("Λ. " ++ showTerm_helper PrecOuter e)
+  | App e1 e2 => parens prec PrecInner (showTerm_helper PrecInner e1 ++ " " ++ showTerm_helper PrecApp e2)
+  | TApp e t => parens prec PrecInner (showTerm_helper PrecInner e ++ " [" ++ show t ++ "]")
+  | Tuple es => "<" ++ intersperse ", " (map (showTerm_helper PrecOuter) es) ++ ">"
+  | ProjN i e => parens prec PrecInner ("π" ++ show i ++ " " ++ showTerm_helper PrecApp e)
+  | Num n => show n
+  | If0 c e1 e2 => parens prec PrecApp ("if0 " ++ showTerm_helper PrecOuter c ++ " then " ++ showTerm_helper PrecOuter e1 ++ " else " ++ showTerm_helper PrecOuter e2)
+  | Op op e1 e2 =>
+    let oprec := op_prec op in
+    parens prec oprec (showTerm_helper oprec e1 ++ " " ++ show op ++ " " ++ showTerm_helper oprec e2) 
+  end.
+
+Instance showTerm {I} `{FInt I} `{Show I} : Show Term :=
+  {| show := showTerm_helper PrecOuter
+  |}.
